\documentclass{book}

\input{../import.tex}
\input{../newcommands.tex}
 
\title{\huge{Utledninger}}
\author{
    \large{Martin KjÃ¸llesdal Johnsrud }
    }


\bibliography{master}


\begin{document}

\maketitle
\setlength{\parindent}{0em}
\setlength{\parskip}{0.8em}

\chapter{CHPT}
\section{Leading order Lagrangian}

\subsection{EM contribution only}
Subs $\pi_a / f \rightarrow \pi_a$,
\begin{align}
    \Sigma = \exp{i \pi_a \tau_a}
    & = 1 + i\pi_a\tau_a - \frac{1}{2}\pi_a \pi_a \\
    Q 
    & = \frac{1}{6} + \frac{1}{2} \tau_3
\end{align}

\begin{align}
    Q\Sigma 
    & = 
    \frac{1}{2}
    \left[
        \frac{1}{3} 
        \left(
            1 + i\pi_a\tau_a - \frac{1}{2}\pi_a \pi_a
        \right)
        +
        \tau_3
        \left(
            1 + i\pi_a\tau_a - \frac{1}{2}\pi_a \pi_a
        \right)
    \right] \\
    & = 
    \frac{1}{2}
    \left[
        \frac{1}{3} 
        - \frac{1}{6}\pi_a \pi_a
        + i \pi_a \tau_3 \tau_a
        + \frac{i}{3}  \pi_a \tau_a
        + \tau_3
        - \frac{1}{2}\pi_a \pi_a \tau_3 
    \right] \\
    %
    %
    %
    Q \Sigma^\dagger
    & = 
    \frac{1}{2}
    \left[
        \frac{1}{3} 
        - \frac{1}{6}\pi_a \pi_a
        - i \pi_a \tau_3 \tau_a
        - \frac{i}{3}  \pi_a \tau_a
        +\tau_3
        - \frac{1}{2}\pi_a \pi_a \tau_3 
    \right] 
\end{align}


Using $
\Tr{\tau_a \tau_b \tau_c \tau_d} = 2 (\delta_{ab}\delta_{cd}
 - \delta_{ac}\delta_{bd}
 \delta_{ad}\delta_{cb})
$, and defining $\delta_{ab}^i = \delta_{ai}\delta_{bi}$,

\begin{align}
    \Tr{Q \Sigma Q \Sigma^\dagger}
    & =
    \frac{1}{2^2}
    \Tr{
        \frac{1}{9}
        - 2 \frac{1}{2\cdot 3^2} \pi_a \pi_a
        + \pi_a \pi_a \tau_3 \tau_a\tau_3 \tau_a
        + \frac{1}{8} \pi_a \pi_a
        + 1
        - \pi_a\pi_a
    } \\
    & = 
    \frac{1}{2}
    \left(
        \frac{1}{9}
        + 1
        - \frac{1}{3^2} \pi_a \pi_a
        - \pi_a \pi_a
        + \frac{1}{9} \pi_a \pi_a
        + \pi_a \pi_a(2 \delta_{ab}^3 - \delta_{ab})
    \right) \\
    &
    = \frac{5}{9} - \pi_1^2 - \pi_2^2.
\end{align}'

\subsection{Free energy EM contribution}

\begin{equation}
    \Eff / u_0 = -
    \left( 
        \cos \alpha 
        + \frac{1}{2} \frac{\mu_I^2}{\bar m^2} \sin^2 \alpha 
        + \frac{1}{2} \Delta  \cos^2 \alpha 
    \right)
\end{equation}
Intrdouce $y^2 = \mu_I^2 / \bar m^2 = x^{-2}$. 
\begin{equation}
    -\frac{1}{u_0}\odv{\Eff}{\alpha} = 
    \left(  
        1 + [y^2 - \Delta ]\cos \alpha 
    \right) \sin \alpha = 0.
\end{equation}
New phase at $y = 1 + \Delta$, where
\begin{equation}
    \cos \alpha = \frac{1}{y^2 - \Delta} 
    \implies \sin^2 \alpha = 1 - \frac{1}{(y^2 - \Delta)^2}
\end{equation}
Pressure
\begin{align}
    \tilde p' 
    &= -\Eff/u_0 = \frac{1}{y^2 - \Delta} 
    + \frac{1}{2} y^2 \left( 1 - \frac{1}{(y^2 - \Delta)^2} \right)
    + \frac{1}{2} \Delta \frac{1}{(y^2 - \Delta)^2} \\
    & = \frac{1}{2} y^2 + \frac{1}{y^2 - \Delta}
    - \frac{1}{2} \frac{y^2 + \Delta}{(y^2 - \Delta)^2} \\
    & \frac{1}{2} \left(y^2 + \frac{1}{y^2 - \Delta}\right).
\end{align}
Normalize
\begin{equation}
    p = p' - p'|_{y^2 = (1 - \Delta)}
    = \frac{1}{2} \left( y^2 + \frac{1}{y^2 + \Delta} - 2 - \Delta \right).
\end{equation}
Isospin density
\begin{equation}
    \frac{\mu_I}{u_0} n_I = - \frac{\mu_I}{u_0} \odv{\Eff}{\mu_I}
    = y^2 \sin^2 \alpha.
\end{equation}
Energy density
\begin{align}
    \tilde u &= -\tilde p + \frac{1}{u_0} \mu_I n_I
    = \frac{1}{2} 
    \left(
        y^2 + \frac{1}{y^2 - \Delta} - 2 - \Delta + 2y^2 
        \left[1 -\frac{1}{(y^2 - \Delta)^2}\right]
    \right) \\
    & =
    \frac{1}{2}
    \left(
        y^2
        - \frac{3 y^2  - \Delta}{(y^2 - \Delta)^2}
        + 2 + \Delta 
    \right).
\end{align}


\section{Newtonian stars}

    \begin{equation}
        \dd \left(\frac{u}{n}\right) = - p \dd \left(\frac{1}{n}\right).
    \end{equation}
    Polytrope: $p = K u^\gamma$, internal energy (assuming $\gamma \neq 1$): $u' = u - m n$, where $m$ is particle mass, $n$ particle number density, $p = K (mn)^\gamma (1 + u' / (mn))^\gamma$.
    \begin{align}
        \dd \frac{u}{n}= \dd \frac{u'}{n} =  \frac{1}{n} \dd u' + u'\dd \frac{1}{n}  = - k (m n)^\gamma \left(1 + \frac{u'}{mn}\right)^\gamma \dd \frac{1}{n}\\ 
        \implies \dd u' = \left(\frac{u'}{mn} + k(mn)^{\gamma - 1}[1 + u' /(mn)]^\gamma \right) m \dd n.
    \end{align}
    non-relativistic limit, $u' \ll mn$, we get
    \begin{equation}
        u' = u - mn \sim \frac{k (mn)^\gamma}{\gamma - 1} \sim \frac{p}{\gamma - 1}, 
    \end{equation}
    as $p \sim k (mn)^\gamma$.

\subsection{Energy}
    \begin{equation}
        \Phi = - \frac{G m u}{r}, \quad \odv{p}{r} = - \frac{G m u}{r^2}.
    \end{equation}
    Total kinetic energy is $T$, potential $V$.
    \begin{align}
        T &= 4 \pi \int_0^R\dd r\, r^2 u' = \frac{4 \pi}{\gamma - 1} \int r^2 p,\\
        V &= - 4 \pi \int_0^R \dd r \,  r^2 \frac{G m u}{r} = \int \dd r \, r^3 \odv{p}{r}
        = -3 \cdot 4 \pi \int \dd r\, r^2 p\\ 
        & \implies T = -3 (\gamma - 1) V.
    \end{align}
    With $\dd m = 4 \pi r^2 u \dd r$, we get
    \begin{equation}
        I = 4 \pi \int \dd r^2 r^2 p = \int \dd m \frac{p}{u} = - \int \dd \left(\frac{p}{u}\right) m,
    \end{equation}
    where we integrated by parts and used $m(0) = p(R)/u(R) = 0$. (assum $\gamma > 1$).
    \begin{equation}
        \dd \frac{p}{u} = \frac{\gamma - 1}{\gamma} \frac{\dd p}{u} = -\frac{\gamma - 1}{\gamma} \frac{Gm}{r^2} \dd r,
    \end{equation}
    as $\gamma p \dd u = \dd p u$. With this, we integrate by parts to obtain
    \begin{equation}
        I = \frac{\gamma - 1}{\gamma} \int \dd r \frac{G m^2}{r}
        = \frac{\gamma - 1}{\gamma} \left[  - \int \dd \left(\frac{1}{r}\right) Gm^2\right]
        = -\frac{\gamma - 1}{\gamma} \left[\frac{GM^2}{R} - 2 \int \dd m \frac{G m}{r} \right]
    \end{equation}
    using $\dd m = 4 \pi r^2 u$, we get
    \begin{equation}
        \int \dd m \frac{G m}{r} = 4\pi\int \dd r\, r G m u = -3I, \implies I = \frac{5\gamma - 6}{\gamma - 1} \frac{GM^2}{R}
    \end{equation}
    Combining $E = T + V$, we get
    \begin{equation}
        E = - \frac{3 \gamma  - 4}{5 \gamma - 6} \frac{G M}{R^2}
    \end{equation}

\end{document}
 